define  Min

src/Tree.lean
@@ -1,6 +1,6 @@
-import reducibility function  data.list.basic
+import lib 
 
-open encodable denumerable t_reducible
+open encodable denumerable
 
 attribute [simp] set.set_of_app_iff
 
@@ -22,32 +22,101 @@ instance : ∀ n, decidable_eq (Tree' n)
 
 def Tree (n : ℕ) := Tree' (n + 1)
 
-def branch {n} (η : Tree n) := { μ : Tree n // μ ⊂ᵢ η }
+instance : has_zero (zero ⊕ infinity) := ⟨sum.inl zero.zero⟩
 
-instance {n} {η : Tree n} : has_lt (branch η) := ⟨λ x y, x.val ⊂ᵢ y.val⟩
-instance {n} {η : Tree n} : has_le (branch η) := ⟨λ x y, x.val <:+ y.val⟩
+notation `∞` := sum.inl infinity.infinity
 
 instance {n} : has_ssubset (Tree n) := ⟨λ x y, x ⊂ᵢ y⟩
 instance {n} : has_subset (Tree n) := ⟨λ x y, x <:+ y⟩
 
+def branch {n} (η : Tree n) := { μ : Tree n // μ ⊂ᵢ η }
+
+instance {n} {η : Tree n} : linear_order (branch η) :=
+{ le := λ x y, x.val <:+ y.val,
+  lt := λ x y, x.val ⊂ᵢ y.val,
+  le_refl := λ μ, by simp,
+  le_trans := λ μ₁ μ₂ μ₃, list.is_suffix.trans,
+  lt_iff_le_not_le := λ μ₁ μ₂, by { simp[list.is_initial_iff_suffix], intros h₁,
+    split,
+    { contrapose, simp, intros h₂, exact list.suffix_antisymm h₁ h₂ },
+    { contrapose, simp, intros eqn, simp[eqn] } },
+  le_antisymm := λ μ₁ μ₂ eqn₁ eqn₂, subtype.eq (list.suffix_antisymm eqn₁ eqn₂),
+  le_total := λ μ₁ μ₂, by { simp[has_le.le, preorder.le],
+    have h₁ := (list.is_initial_iff_suffix.mp μ₁.property).1,
+    have h₂ := (list.is_initial_iff_suffix.mp μ₂.property).1,
+    exact list.suffix_or_suffix_of_suffix h₁ h₂ },
+  decidable_le := λ μ₁ μ₂, list.decidable_suffix μ₁.val μ₂.val,
+  decidable_eq := subtype.decidable_eq,
+  decidable_lt := λ μ₁ μ₂, list.is_initial_decidable μ₁.val μ₂.val, }
+
+def Tree.branches {n} (η : Tree n) : list (branch η) :=
+(list.range_r η.length).pmap (λ m (h :m < η.length), (⟨η↾*m, list.is_initial_of_lt_length h⟩ : branch η))
+(λ _, by simp)
+-- η.branches = [ ... η↾*2, η↾*1, η↾*0]
+
 namespace branch
 
-def branch_range {n} (η : Tree n) : list (branch η) :=
-(list.range η.length).pmap (λ m (h :m < η.length), ⟨η↾*m, list.is_initial_of_lt_length h⟩) (λ _, by simp)
+@[simp] def cons' {n} {η : Tree n} {a} (μ : branch η) : branch (a :: η) :=
+⟨μ.val, μ.property.trans (η.is_initial_cons _)⟩
 
-lemma nodup_branch_range {n} (η : Tree n) : (branch_range η).nodup :=
+@[simp] def extend {n} {η₁ η₂ : Tree n} (s : η₁ <:+ η₂) (μ : branch η₁) : branch η₂ :=
+⟨μ.val, list.suffix_of_is_initial_is_initial μ.property s⟩
+
+@[simp] lemma extend_id {n} {η : Tree n} {s} : @extend _ η η s = id :=
+funext (by simp)
+
+@[simp] lemma branches_nil {n} : @Tree.branches n [] = [] := rfl
+
+@[simp] lemma branches_cons {n} (η : Tree n) (x) : Tree.branches (x :: η) = ⟨η, by simp⟩ :: η.branches.map cons' :=
+by { simp[Tree.branches, list.map_pmap], apply list.pmap_congr, simp,
+     intros m eqn₁ eqn₂, simp [list.initial_cons eqn₂] }
+
+lemma branches_suffix_of_suffix {n} {μ₁ μ₂ : Tree n} (s : μ₁ <:+ μ₂) :
+  μ₁.branches.map (branch.extend s) <:+ μ₂.branches :=
+begin
+  rcases s with ⟨l, h⟩,
+  induction l with x l IH generalizing μ₁ μ₂,
+  { simp at h, rcases h with rfl, simp },
+  { simp at h, rcases h with rfl, simp,
+    have : μ₁.branches.map (λ ν₁, (⟨ν₁.val, _⟩ : branch (x :: (l ++ μ₁))))
+      <:+ list.map cons' (Tree.branches (l.append μ₁)),
+    { have := list.map_suffix cons' (@IH μ₁ (l.append μ₁) rfl), simp[function.comp] at this, exact this },
+    exact this.trans (list.suffix_cons _ _) }
+end
+
+@[simp] lemma branches_length {n} {μ : Tree n} : μ.branches.length = μ.length := by simp[Tree.branches]
+
+lemma branches_rnth {n} {μ : Tree n} {i : ℕ} (h : i < μ.length)  :
+  μ.branches.rnth i = some ⟨μ↾*i, list.is_initial_of_lt_length h⟩ :=
+begin
+  have : μ.branches.rnth i = μ.branches.nth (list.length μ - 1 - i),
+  { have := @list.rnth_eq_nth_of_lt _ μ.branches i (by simp[h]), simp at this, exact this },
+  rw this, simp[Tree.branches, list.nth_pmap],
+  refine ⟨i, _, rfl⟩,
+  have := @list.rnth_eq_nth_of_lt _ (list.range_r (list.length μ)) i (by simp[h]), simp[h] at this,
+  exact eq.symm this
+end
+
+lemma branches_ordered {n} : ∀ (μ : Tree n), μ.branches.ordered (<)
+| []       := by simp
+| (x :: η) := by simp; exact ⟨list.ordered_map cons' (λ x y lt, lt) (branches_ordered η), λ η₀ mem, η₀.property⟩
+
+lemma nodup_Tree.branches {n} (η : Tree n) : (Tree.branches η).nodup :=
 list.nodup_pmap
   (λ m₁ eqn₁ m₂ eqn₂ eqn, by { simp at eqn, have : (η↾*m₁).length = m₁, from list.initial_length eqn₁,
        simp [eqn, list.initial_length eqn₂] at this, simp[this] })
-  (list.nodup_range _)
+  (list.nodup_range_r _)
 
 def branch_univ {n} (η : Tree n) : finset (branch η) :=
-⟨branch_range η, nodup_branch_range η⟩
+⟨Tree.branches η, nodup_Tree.branches η⟩
 
-@[simp] lemma mem_fin_range {n} {η : Tree n} (η₀ : branch η) : η₀ ∈ branch_univ η :=
+@[simp] lemma branches_complete {n} {η : Tree n} (η₀ : branch η) : η₀ ∈ η.branches :=
 list.mem_pmap.2 ⟨η₀.val.length, by { simp[branch_univ],
 refine ⟨list.is_initial_length η₀.property, _⟩, apply subtype.ext, simp,
 exact list.eq_initial_of_is_initial η₀.property }⟩
+
+@[simp] lemma mem_fin_range {n} {η : Tree n} (η₀ : branch η) : η₀ ∈ branch_univ η :=
+branches_complete _
 
 instance {n} (η : Tree n) : fintype (branch η) :=
 ⟨branch_univ η, mem_fin_range⟩
@@ -55,7 +124,7 @@ instance {n} (η : Tree n) : fintype (branch η) :=
 def branch_univ' {n} (η : Tree n) : finset (Tree n) := (branch_univ η).image subtype.val  
 
 @[simp] lemma branch_univ_card {n} (η : Tree n) : (branch_univ η).card = η.length :=
-by simp[branch_univ, branch_range]
+by simp[branch_univ, Tree.branches]
 
 @[simp] lemma branch_univ'_card {n} (η : Tree n) : (branch_univ' η).card = η.length :=
 by { have : (branch_univ' η).card = (branch_univ η).card,
@@ -65,27 +134,6 @@ by { have : (branch_univ' η).card = (branch_univ η).card,
 instance {n} {η : Tree n} : has_coe (branch η) (Tree n) :=
 ⟨subtype.val⟩
 
-lemma linear {n} {η : Tree n} {μ₁ μ₂ : branch η} :
-  μ₂ ≤ μ₁ ↔ ¬μ₁ < μ₂ :=
-begin
-  split,
-  { simp[has_lt.lt, has_le.le, list.suffix_iff_is_initial], rintros (h | h),
-    { intros h₁, have := h.trans h₁, simp* at* },
-    { simp[h] } },
-  { simp[has_lt.lt, has_le.le, list.is_initial_iff_suffix], intros h,
-    rcases list.is_initial_iff_suffix.mp μ₁.property with ⟨h₁, eqn₁⟩,
-    rcases list.is_initial_iff_suffix.mp μ₂.property with ⟨h₂, eqn₂⟩,
-    have : μ₁.val <:+ μ₂.val ∨ μ₂.val <:+ μ₁.val, from list.suffix_or_suffix_of_suffix h₁ h₂,
-    cases this,
-    { simp[h this] }, { exact this } }
-end
-
-lemma le_lt {n} {η : Tree n} {μ₁ μ₂ : branch η} :
-  μ₁ ≤ μ₂ ↔ μ₁ < μ₂ ∨ μ₁ = μ₂ :=
-by { simp[has_lt.lt, has_le.le],
-     have := @list.suffix_iff_is_initial _ (↑μ₁) (↑μ₂), rw [←subtype.ext_iff] at this,
-     exact this }
-
 end branch
 
 structure Path (n : ℕ) :=
@@ -93,6 +141,12 @@ structure Path (n : ℕ) :=
 (mono : ∀ m, path m <:+ path (m + 1))
 
 namespace Path
+
+def trivialPath_aux {i : ℕ} : ℕ → Tree i
+| 0       := []
+| (n + 1) := ∞ :: trivialPath_aux n
+
+instance (i) : nonempty (Path i) := ⟨⟨trivialPath_aux, by simp[trivialPath_aux]⟩⟩
 
 variables {i : ℕ} (Λ : Path i)
 
@@ -108,9 +162,65 @@ end
 
 end Path
 
-def branch.cons' {n} {η : Tree n} {a} (μ : branch η) : branch (a :: η) :=
-⟨μ.val, μ.property.trans (η.is_initial_cons _)⟩
+structure strategy (R : Type*) :=
+(par₀ : Tree 0 → ℕ)
+(par₁ : Tree 1 → ℕ)
+(requirement : Tree 1 × ℕ → R)
+(computation : Tree 0 × R → Tree 0 × R → Prop)
+(inf : Tree 1 × ℕ → Tree 1 × ℕ → Tree 1 × ℕ)
 
-instance : has_zero (zero ⊕ infinity) := ⟨sum.inl zero.zero⟩
+def out {n} : Π {η : Tree n}, branch η → infinity ⊕ Tree' n
+| []       ⟨μ, μ_p⟩ := by exfalso; simp* at*
+| (ν :: η) ⟨μ, μ_p⟩ := if h : μ ⊂ᵢ η then out ⟨μ, h⟩ else ν
 
-notation `∞` := sum.inl infinity.infinity
+lemma out_eq_iff {n} : ∀ {η : Tree n} {μ : branch η} {ν}, out μ = ν ↔ ν :: μ.val <:+ η
+| []       ⟨μ, μ_p⟩ _  := by exfalso; simp* at*
+| (ν :: η) ⟨μ, μ_p⟩ ν' :=
+    by { simp, have : μ = η ∨ μ ⊂ᵢ η, from list.is_initial_cons_iff.mp μ_p, cases this,
+         { rcases this with rfl, simp[out], exact eq_comm },
+         { simp[out, this],
+           have IH : out ⟨μ, this⟩ = ν' ↔ ν' :: μ <:+ η, from @out_eq_iff η ⟨μ, this⟩ ν', rw IH,
+           split,
+           { intros h, refine list.suffix_cons_iff.mpr (or.inr h) },
+           { intros h, have C := list.suffix_cons_iff.mp h, cases C,
+             { exfalso, simp at C, rcases C with ⟨_, rfl⟩, simp at this, exact this },
+             { exact C } } } }
+
+lemma suffix_out_cons {n} {η : Tree n} (μ : branch η) : out μ :: μ.val <:+ η :=
+by { have := @out_eq_iff n η μ (out μ), simp* at* }
+
+lemma out_cons'_eq {n} {η : Tree n} (ν) (μ : branch η)  :
+  @out n (ν :: η) μ.cons' = out μ :=
+by { simp[out, branch.cons'], intros h, exfalso, have := h μ.property, exact this }
+
+lemma out_cons'_eq' {n} {η : Tree n} (ν) (μ : branch η) {h : μ.val ⊂ᵢ ν :: η} :
+  @out n (ν :: η) ⟨μ.val, h⟩ = out μ :=
+by { simp[out, branch.cons'], intros h, exfalso, have := h μ.property, exact this }
+
+lemma suffix_out_eq {n} : ∀ {η₁ η₂: Tree n} {μ₁ : branch η₁} {μ₂ : branch η₂}
+  (h₁ : μ₁.val = μ₂.val) (h₂ : η₂ <:+ η₁), out μ₁ = out μ₂ :=
+begin
+  suffices : ∀ (l : list _) {η₁ η₂: Tree n} {μ₁ : branch η₁} {μ₂ : branch η₂}
+    (h₁ : μ₁.val = μ₂.val) (h₂ : l.reverse ++ η₂ = η₁), out μ₁ = out μ₂,
+  { intros η₁ η₂ μ₁ μ₂ h₁ h₂, rcases h₂ with ⟨l, h₂⟩,
+    exact this l.reverse h₁ (by simp[h₂]) },
+  intros l η₁ η₂ μ₁ μ₂ h₁ h₂,
+  induction l with ν l IH generalizing η₁ η₂,
+  { simp at h₂, rcases h₂ with rfl, congr, exact subtype.eq h₁ },
+  { simp at h₂,
+    let μ₂' : branch (ν :: η₂) := ⟨μ₂.val, μ₂.property.trans (by simp)⟩,
+    have h₁' : μ₁.val = μ₂'.val, { simp[μ₂', h₁] },
+    have eqn₁ : out μ₁ = out μ₂', from IH h₁' h₂,
+    have eqn₂ : out μ₂' = out μ₂, from out_cons'_eq' ν μ₂,
+    simp[eqn₁, eqn₂] }
+end
+
+lemma rnth_eq_iff_out {n} {η : Tree n} {ν} {m : ℕ} :
+  η.rnth m = some ν ↔ ν :: η↾*m <:+ η :=
+list.rnth_eq_iff_suffix_cons_initial
+
+lemma rnth_eq_some_out {n} {η : Tree n} {μ : branch η} {m : ℕ} (h : m < η.length) :
+  η.rnth m = some (out (⟨η↾*m, list.is_initial_of_lt_length h⟩ : branch η)) :=
+rnth_eq_iff_out.mpr (suffix_out_cons ⟨η↾*m, list.is_initial_of_lt_length h⟩)
+
+
